search_requests.dfy
@@ -11,10 +11,11 @@
     description: 'efwlneefw' } ]
 */
 
-class RowDataPacket {
+class {:autocontracts} RowDataPacket 
+{
     var id: int;
     var userID: int;
-    var event_name string;
+    var event_name: string;
     var event_date: string; // ??? date
     var event_time: string; // ??? time
     var deadline: string; // ??? date
@@ -27,4 +28,90 @@ class RowDataPacket {
     var additional_info: string;
     var last_modified: string; // ??? datetime
     var status: int;
+    
+    predicate Valid() {
+      |deadline| == |event_date| == 10
+    }
+    
+    method init(id: int, userID: int, event_name: string, event_date: string, event_time: string, deadline: string, suburb: string, event_type: string, 
+                no_people: int, food_quality: string, budget: real, choice: string, additional_info: string, last_modified: string, status: int)
+        requires |deadline| == |event_date| == 10;
+        modifies this;
+        ensures this.id==id && this.userID==userID && this.event_name==event_name && this.event_date==event_date && 
+            this.event_time==event_time && this.deadline==deadline && this.suburb==suburb && this.event_type==event_type && 
+            this.no_people==no_people && this.food_quality==food_quality && this.budget==budget && this.choice==choice && 
+            this.additional_info==additional_info && this.last_modified==last_modified && this.status==status
+    {
+      this.id:= id;
+      this.userID:= userID;
+      this.event_name:= event_name;
+      this.event_date:= event_date;
+      this.event_time:= event_time;
+      this.deadline:= deadline;
+      this.suburb:= suburb;
+      this.event_type:= event_type;
+      this.no_people:= no_people;
+      this.food_quality:= food_quality;
+      this.budget:= budget;
+      this.choice:= choice;
+      this.additional_info:= additional_info;
+      this.last_modified:= last_modified;
+      this.status:= status;
+    }
 }
+
+method strcmp(a:string, b:string) returns (result: bool)
+requires |a| == |b|
+ensures result == 1 || result == -1
+ensures result == 1 ==> forall j :: 0<=j<|a| ==> a[j]==b[j]
+ensures result == -1 ==> exists i :: 0<=i<|a| && (a[i] != b[i] && (forall j :: 0<=j<i ==> a[j]==b[j]))
+{
+    var i:int;
+    i:=0;
+    while (i < |a| && a[i] == b[i])
+        invariant 0<=i<=|a|
+        invariant forall k::0<=k<i ==> a[k]==b[k]
+    {
+        i:=i+1;  
+    }
+    if (i == |a|) {
+        result:=1;
+    }
+    else {
+        if (a[i] != b[i]) {
+        result:=-1;
+        }
+    }
+}
+
+predicate str_match(a: string, b: string)
+    requires |a| == |b|
+{   strcmp(a,b) == 1     }
+
+predicate str_not_match(a: string, b: string)
+{   strcmp(a,b) == -1   }
+
+
+method Search(a: array<RowDataPacket>, key: string) returns(b: array<RowDataPacket>)
+modifies b
+requires a.Length > 1
+ensuires 
+ensures forall k:: 0<=k<b.Length ==> b[k].event_type = key
+{
+    var i, j, cmp: int
+    i:=0;
+    j:=0;
+    while i<a.Length
+        invariant 0<=i<=a.Length
+        invariant forall k:: j<k<i ==> a[k]!=key
+    {
+        cmp:=strcmp(a[i],key)
+        if (cmp == 1){ 
+            b[j]:= a[i];
+            j:=j+1; 
+        }
+        i:=i+1;
+    }
+    return b;
+}    
+
